Move bv smtlib definitions to SMT_word

src/HOL/CVC/cvc5_dsl_rewrites/BV_Rewrites_Lemmas.thy
@@ -1,535 +1,6 @@
 theory BV_Rewrites_Lemmas
-  imports Dsl_Nary_Ops "HOL-Library.Word" Word_Lib.More_Word "HOL-Library.Log_Nat"  "HOL-Library.Word" "HOL.Real"
-"HOL-Library.Sublist" "HOL-Library.Log_Nat"
+  imports Dsl_Nary_Ops "HOL-Library.Word" Word_Lib.More_Word "HOL-Library.Log_Nat" "HOL.Real" "HOL-Library.Sublist" "HOL-CVC.SMT_Word"
 begin
-
-(*imported from various places*)
-
-(*IEEE_Float_Extend_Integer*)
-lemma nat_bit_shift_add_bound:
-  fixes e f :: nat
-  assumes LF: "f<2^F"
-      and LE: "e<2^E"
-  shows "f+e*2^F < 2^(E+F)"
-proof -
-  from LE have "e \<le> 2^E - 1" by simp
-  hence "e*2^F \<le> (2^E - 1) * 2^F" by simp
-  also have "\<dots> = 2^(E+F) - 2^F" by (simp add: power_add algebra_simps)
-  finally have "e * 2 ^ F \<le> 2 ^ (E + F) - 2 ^ F" .
-  thus ?thesis using LF
-    by (metis LE add.commute nat_add_offset_less)
-qed
-
-lemma int_bit_shift_add_bound:
-  fixes e f :: int
-  assumes LF: "f<2^F"
-      and LE: "e<2^E"
-  shows "f+e*2^F < 2^(E+F)"
-proof -
-  from LE have "e \<le> 2^E - 1" by simp
-  hence "e*2^F \<le> (2^E - 1) * 2^F" by simp
-  also have "\<dots> = 2^(E+F) - 2^F" by (simp add: power_add algebra_simps)
-  finally have "e * 2 ^ F \<le> 2 ^ (E + F) - 2 ^ F" .
-  thus ?thesis using LF by linarith
-qed
-  
-lemma uint_bit_shift_add_bound:
-  fixes f :: "'f::len word"
-    and e :: "'e::len word"
-  shows "uint (f) + uint (e) * 2 ^ LENGTH('f) < 2^(LENGTH('e) + LENGTH('f))"
-  apply (rule int_bit_shift_add_bound)
-  by auto
-
-lemma unat_bit_shift_add_bound:
-  fixes f :: "'f::len word"
-    and e :: "'e::len word"
-  shows "unat (f) + unat (e) * 2 ^ LENGTH('f) < 2^(LENGTH('e) + LENGTH('f))"
-  apply (rule nat_bit_shift_add_bound)
-  by auto
-
-lemma unat_pow_le_intro:
-  "LENGTH('a) \<le> n \<Longrightarrow> unat (x :: 'a :: len word) < 2 ^ n"
-  by (metis lt2p_lem not_le of_nat_le_iff of_nat_numeral semiring_1_class.of_nat_power uint_nat)
-
-lemma unat_word_cat_eq:
-  fixes w\<^sub>1 :: "'l\<^sub>1::len word"
-  fixes w\<^sub>2 :: "'l\<^sub>2::len word"
-  assumes "LENGTH('l\<^sub>1) + LENGTH('l\<^sub>2) \<le> LENGTH('l\<^sub>3)"
-  shows "unat (word_cat w\<^sub>1 w\<^sub>2 :: 'l\<^sub>3::len word) = unat w\<^sub>2 + unat w\<^sub>1 * 2^LENGTH('l\<^sub>2)"  
-proof -
-  have [simp]: "LENGTH('l\<^sub>2) < LENGTH('l\<^sub>3)"
-    using assms 
-    by (metis add_diff_cancel_right' add_leD2 diff_is_0_eq' le_neq_implies_less len_not_eq_0)
-  have B2: "unat w\<^sub>2 + unat w\<^sub>1 * unat ((2::'l\<^sub>3 word) ^ LENGTH('l\<^sub>2)) < 2 ^ LENGTH('l\<^sub>3)"
-    apply (simp)
-    apply (rule order.strict_trans2[OF unat_bit_shift_add_bound])
-    using assms by simp
-
-  have B1: "unat w\<^sub>1 * unat ((2::'l\<^sub>3 word) ^ LENGTH('l\<^sub>2)) < 2 ^ LENGTH('l\<^sub>3)" 
-    using B2 by linarith
-          
-  show ?thesis  
-    apply (simp add: word_cat_eq' concat_bit_eq take_bit_eq_mod push_bit_eq_mult)
-    apply (simp add: unat_word_ariths unat_ucast_upcast B1 B2)
-    by (metis B2 \<open>LENGTH('l\<^sub>2) < LENGTH('l\<^sub>3)\<close> add.commute add_leD2 add_lessD1 assms nat_mod_eq'
-        unat_pow_le_intro unat_power_lower unat_ucast)
-qed
-(*end of stolen*)
-
-(* SMT-LIB bit-vector definitions *)
-
-definition smt_extract where
-  \<open>smt_extract j i w = slice i (take_bit (Suc j) w)\<close>
-
-lemma unat_smt_extract:
-  fixes x::"'a::len word"
-  shows  "i \<le> j \<Longrightarrow> j < size x \<Longrightarrow> LENGTH('b) = j + 1 - i
- \<Longrightarrow> unat ((smt_extract j i (x::'a::len word))::'b::len word)
-   = drop_bit i (take_bit (Suc j) (unat x))"
-  apply (cases "i=0")
-proof-
-  assume a0: "i = (0::nat)" and a1: "i \<le> j" "j < size x" "LENGTH('b) = j + 1 - i"
-  then have t0: "LENGTH('b) \<le> LENGTH('a)"
-    by (simp add: size_word.rep_eq)
-  have "unat (smt_extract j i x::'b::len word) = unat (ucast (take_bit (Suc j) x ::'a::len word)::'b::len word)"
-   unfolding smt_extract_def slice_def slice1_def
-   by (simp add: a0)
-  also have "... = unat (take_bit (Suc j) x ::'a::len word)"
-    by (simp add: a1 a0 unsigned_take_bit_eq unsigned_ucast_eq)
-  also have "... = take_bit (Suc j) (unsigned x)" 
-    using Word.semiring_bit_operations_class.unsigned_take_bit_eq
-    by auto
-  finally show "unat ((smt_extract j i (x::'a::len word))::'b::len word) = drop_bit i (take_bit (Suc j) (unat x))"
-    using a0 by force
-next
-  assume a0: "i \<noteq> (0::nat)" and a1: "i \<le> j" "j < size x" "LENGTH('b) = j + 1 - i"
-  then have t0: "LENGTH('b) \<le> LENGTH('a)"
-    by (metis Suc_eq_plus1 Suc_leI diff_le_self le_trans size_word.rep_eq)
-  have t1: "i < LENGTH('a)"
-    by (metis a1(1,2) dual_order.strict_trans2 size_word.rep_eq)
-  have "unat (smt_extract j i x::'b::len word) = unat (ucast (drop_bit i (take_bit (Suc j) x))::'b::len word)"
-    unfolding smt_extract_def slice_def slice1_def
-    using a0 t1 by force
-  also have "... = unat (drop_bit i (take_bit (Suc j) x))"
-    by (metis (no_types, lifting) Suc_eq_plus1 a1(3) drop_bit_take_bit min.idem take_bit_take_bit unsigned_take_bit_eq unsigned_ucast_eq)
-  also have "... = drop_bit i (unsigned (take_bit (Suc j) x))" 
-    using unat_drop_bit_eq by blast
-  also have "... = drop_bit i (take_bit (Suc j) (unsigned x))" 
-    by (simp add: unsigned_take_bit_eq)
-  finally show "unat ((smt_extract j i (x::'a::len word))::'b::len word) = drop_bit i (take_bit (Suc j) (unat x))"
-    by simp
-qed
-
-lemma uint_smt_extract:
-  fixes x::"'a::len word"
-  shows  "i \<le> j \<Longrightarrow> j < size x \<Longrightarrow> LENGTH('b) = j + 1 - i
- \<Longrightarrow> uint ((smt_extract j i (x::'a::len word))::'b::len word)
-   = drop_bit i (take_bit (Suc j) (unsigned x))"
-  apply (subst uint_nat)
-  apply (simp add: unat_smt_extract)
-  by (metis Word.of_nat_unat of_nat_drop_bit take_bit_of_nat)
-
-lemma sint_smt_extract:
-  fixes x::"'a::len word"
-  shows  "i \<le> j \<and> j < size x \<and> LENGTH('b) = j + 1 - i
- \<Longrightarrow> sint ((smt_extract j i (x::'a::len word))::'b::len word)
-= signed_take_bit (LENGTH('b::len) - Suc (0::nat)) (drop_bit i (take_bit (Suc j) (unsigned x)))"
-  apply (subst sint_uint)
-  by (simp add: uint_smt_extract)
-
-definition replicate_nat :: \<open>_ \<Rightarrow> _ \<Rightarrow> nat\<close> where
- \<open>replicate_nat i s = (\<Sum>k=0..(i-1). 2^(s*k))\<close>
-
-lemma replicate_nat_Suc[simp]:
-  \<open>i > 0 \<Longrightarrow> replicate_nat (Suc i) s = replicate_nat i s + (2::nat) ^ (i*s)\<close>
-  by (cases i) (auto simp: replicate_nat_def)
-
-definition word_repeat :: \<open>nat \<Rightarrow> 'a :: len word \<Rightarrow> 'b :: len word\<close> where
- \<open>word_repeat i n = (THE x :: 'b::len word. LENGTH('b) = i * size n \<and> unat x = replicate_nat i (size n) * (unat n))\<close>
-
-lemma ex_unat_nat: "n < 2^ (LENGTH('a)) \<Longrightarrow> \<exists>x :: 'a:: len word. unat x = n"
-  using of_nat_inverse by blast
-
-lemma replicate_nat_le: \<open>i \<ge> 1 \<Longrightarrow> replicate_nat i (size n) * unat n < 2 ^ (i * size n)\<close>
-  apply (induction i)
-  subgoal by auto
-  subgoal for i
-    apply (cases i)
-    apply (auto simp: replicate_nat_def)
-    apply (simp add: wsst_TYs(3))
-    by (simp add: distrib_left mult.commute nat_bit_shift_add_bound wsst_TYs(3))
-  done
-
-lemma word_repeat_unique:
-  \<open>LENGTH('b) = i * size n \<and> unat a = replicate_nat i (size n) * unat n \<Longrightarrow>
-  LENGTH('b::len) = i * size n \<and> unat x = replicate_nat i (size n) * unat n \<Longrightarrow>
-  x = a\<close>
-  using word_eq_iff_unsigned
-  by metis
-
-lemma ex_word_repeat:
-  fixes n :: \<open>'a :: len word\<close>
-  assumes \<open>LENGTH('b) = i * size n\<close> "i \<ge> 1" 
-  shows \<open>\<exists>x::'b::len word. unat x = replicate_nat i (size n) * (unat n)\<close>
-  using assms apply -
-  by (rule ex_unat_nat) (auto intro: replicate_nat_le)
-
-lemma word_repeat_prop:
-  \<open>i\<ge>1 \<Longrightarrow> LENGTH('b) = i * size n \<Longrightarrow> unat ((word_repeat i n) :: 'b :: len word) = replicate_nat i (size n) * (unat n)\<close>
-  using ex_word_repeat[of i n, where 'b='b]
-    theI[where P = \<open>\<lambda>x :: 'b::len word. LENGTH('b) = i * size n \<and> unat x = replicate_nat i (size n) * (unat n)\<close>,
-    unfolded word_repeat_def[symmetric]]
-    word_repeat_unique[where 'b='b]
-  by fast
-
-lemma word_repeat_alt_def:
-  assumes \<open>LENGTH('b) = i * size n\<close> \<open>i \<ge> 1\<close>
-  shows \<open>word_repeat i n = (a::'b ::len word) \<longleftrightarrow> (unat a = replicate_nat i (size n) * unat n)\<close>
-proof -
-  have \<open>LENGTH('b) = i * size n \<Longrightarrow> i \<ge> 1 \<Longrightarrow>  word_repeat i n = (a::'b ::len word) \<longleftrightarrow> (LENGTH('b) = i * size n \<and> unat a = replicate_nat i (size n) * unat n)\<close>
-    apply (subst eq_commute[of _ a])
-    apply (subst theI_unique[where P = \<open>\<lambda>x :: 'b::len word. LENGTH('b) = i * size n \<and> unat x = replicate_nat i (size n) * (unat n)\<close>,
-      unfolded word_repeat_def[symmetric], of a])
-    subgoal
-      apply (subst Ex1_def)
-      using
-        ex_word_repeat[of i n, where 'b='b]
-        word_repeat_unique[of i n, where 'b='b]
-      by blast
-    subgoal by auto
-    done
-  then show ?thesis
-    using assms by fast
-qed
-
-lemma word_repeat_word_cat:
-  fixes n :: "'a :: len word"
-  assumes \<open>LENGTH('b::len) = Suc i * size n\<close> \<open>i > 0\<close>
-    \<open>LENGTH('c::len) = i * size n\<close>
-  shows \<open>(word_repeat (Suc i) n :: 'b word) = word_cat (n :: 'a word) (word_repeat i n :: 'c word)\<close>
-  supply [[show_sorts,show_types]]
-  apply (subst word_repeat_alt_def)
-  subgoal using assms by auto
-  subgoal by auto
-    apply (subst unat_word_cat_eq)
-    subgoal using assms by (auto simp: word_size)
-    apply (subst word_repeat_prop)
-    subgoal using assms by auto
-    subgoal using assms by auto
-      apply (subst replicate_nat_Suc)
-    subgoal using assms by auto
-    subgoal using assms by (auto simp: algebra_simps word_size)
-    done
-
-definition smt_repeat :: "nat \<Rightarrow> 'a::len word \<Rightarrow> 'b::len word" where
-  \<open>smt_repeat i x = (if i = 0 then (ucast x::'b::len word) else word_repeat i x)\<close>
-
-definition smt_comp :: "'a::len word \<Rightarrow> 'a::len word \<Rightarrow> 1 word" where
-  \<open>smt_comp x y = (if (x = y) then 1 else 0)\<close>
-
-lemma smt_comp_cast_0 [simp]:
-  assumes "x = y"
-  shows "unat (smt_comp x y) = 1"
-        "uint (smt_comp x y) = 1"
-        "sint (smt_comp x y) = -1"
-  by (simp_all add: smt_comp_def assms)
-
-lemma smt_comp_cast_1 [simp]:
-  assumes "x \<noteq> y"
-  shows "unat (smt_comp x y) = 0"
-        "uint (smt_comp x y) = 0"
-        "sint (smt_comp x y) = 0"
-  by (simp_all add: smt_comp_def assms)
-
-definition smt_redor :: "'a::len word \<Rightarrow> 1 word" where
-  \<open>smt_redor x = not (smt_comp x 0)\<close>
-
-lemma smt_redor_cast_0 [simp]:
-  assumes "x = 0"
-  shows "unat (smt_redor x) = 0"
-        "uint (smt_redor x) = 0"
-        "sint (smt_redor x) = 0"
-  by (simp_all add: smt_redor_def smt_comp_def assms)
-
-lemma smt_redor_cast_1 [simp]:
-  assumes "x \<noteq> 0"
-  shows "unat (smt_redor x) = 1"
-        "uint (smt_redor x) = 1"
-        "sint (smt_redor x) = -1"
-    apply (simp_all add: smt_redor_def smt_comp_def assms)
-  by (simp_all add: unsigned_minus_1_eq_mask)
-
-definition smt_redand :: "'a::len word \<Rightarrow> 1 word" where
-  \<open>smt_redand x = smt_comp x (not (0::'a word))\<close>
-
-lemma smt_redand_cast_0 [simp]:
-  assumes "x \<noteq> -1"
-  shows "unat (smt_redand x) = 0"
-        "uint (smt_redand x) = 0"
-        "sint (smt_redand x) = 0"
-  by (simp_all add: smt_redand_def smt_comp_def assms)
-
-lemma smt_redand_cast_1 [simp]:
-  assumes "x = -1"
-  shows "unat (smt_redand x) = 1"  
-        "uint (smt_redand x) = 1"
-        "sint (smt_redand x) = -1"
-  by (simp_all add: smt_redand_def smt_comp_def assms)
-
-(*'c is 'a + 1*)
-definition smt_uaddo :: "'c::len itself \<Rightarrow> 'a::len word \<Rightarrow> 'b::len word \<Rightarrow> bool" where
-"smt_uaddo TYPE('c) x y = (smt_extract (size x - 1) (size x - 1)
- ((Word.word_cat (0::1 word) x) + (Word.word_cat (0::1 word) y) :: 'c::len word) = (1:: 1 word))"
-
-definition smt_saddo :: "'a::len word \<Rightarrow> 'a::len word \<Rightarrow> bool" where
-"smt_saddo x y = 
-(let sign0=smt_extract (size x - 1) (size x - 1) x in
- let sign1=smt_extract (size x - 1) (size x - 1) y in
- let signa=smt_extract (size x - 1) (size x - 1) (x+y) in
- let both_neg=((sign0 = (1::1 word)) \<and> (sign1 = (1::1 word))) in
- let both_pos=((sign0 = (0::1 word)) \<and> (sign1 = (0::1 word))) in
- let result_neg=(signa = (1::1 word)) in
- let result_pos=(signa = (0::1 word)) in 
-((both_neg \<and> result_pos) \<or> (both_pos \<and> result_neg))
-)"
-
-definition smt_sdivo :: "'c::len itself \<Rightarrow> 'a::len word \<Rightarrow> 'b::len word \<Rightarrow> bool" where
-"smt_sdivo TYPE('c) x y = (x = (word_cat (1::1 word) (0::'c::len word)::'a word) \<and> y = (mask (size y)::'b word))"
-
-definition smt_usubo :: "'c::len itself \<Rightarrow> 'a::len word \<Rightarrow> 'a::len word \<Rightarrow> bool" where
-"smt_usubo TYPE('c) x y = ((smt_extract ((size x)-1) ((size y)-1) ((Word.cast x::'c::len word) - Word.cast y)) = (1::1 word))"
-
-definition smt_ssubo :: "'a::len word \<Rightarrow> 'a::len word \<Rightarrow> bool" where (*TODO*)
-"smt_ssubo x y = 
-(let n = size x in 
-(let xLt0 = ((smt_extract ((size x)-1) ((size x)-1) x) = (1::1 word)) in
-(let yLt0 = ((smt_extract ((size x)-1) ((size x)-1) y) = (1::1 word)) in
-(let sLt0 = ((smt_extract ((size x)-1) ((size x)-1) (x -y)) = (1::1 word)) in
-((xLt0 \<and> \<not>yLt0 \<and> \<not>sLt0) \<or> (\<not>xLt0 \<and> yLt0 \<and> sLt0))))))
-"
-
-lemma "unsigned (if x then y else z) = (if x then unsigned y else unsigned z)"
-  by auto
-declare[[show_types]]
-declare[[show_sorts]]
-
-definition smt_urem :: "'a::len word \<Rightarrow> 'a::len word \<Rightarrow> 'a::len word" where
-"smt_urem s t = (if (unat s = 0) then s
- else of_nat ((unat s) mod (unat t)))"
-
-lemma "uint (smt_urem s t) = (if (s = 0) then (uint s) else int ((unat s) mod (unat t)))"
-proof-
-  have "uint (smt_urem s t) =
-        uint (if (unat s = 0) then s else of_nat ((unat s) mod (unat t)))"
-  unfolding smt_urem_def by simp
-  then have "uint (smt_urem s t) =
-   (if (unat s = 0) then uint s else uint (of_nat ((unat s) mod (unat t))::'a::len word))"
-    by presburger
-  moreover have "uint (of_nat ((unat s) mod (unat t))::'a::len word)
-= int ((unat s) mod (unat t))"
-    by (metis Word.of_nat_unat ucast_id unat_mod)
-  ultimately show ?thesis
-    by (simp add: unsigned_eq_0_iff)
-qed
-
-(* Should be done with bit instead of extract? *)
-definition smt_smod :: "'a::len word \<Rightarrow> 'a::len word \<Rightarrow> 'a::len word" where
-"smt_smod s t =
-(let size_s = size s in
-(let msb_s = smt_extract (size_s-1) (size_s-1) s in 
-(let msb_t = smt_extract (size_s-1) (size_s-1) t in 
-(let abs_s = (if (msb_s = (0::1 word)) then s else -s) in 
-(let abs_t = (if (msb_t = (0::1 word)) then t else -t) in 
-(let u = (smt_urem abs_s abs_t) in 
-(if (u = (0::'a word)) then u
- else if ((msb_s = (0::1 word)) \<and> (msb_t = (0::1 word))) then u
- else if ((msb_s = (1::1 word)) \<and> (msb_t = (0::1 word))) then (-u + t)
- else if ((msb_s = (0::1 word)) \<and> (msb_t = (1::1 word))) then (u + t)
- else -u)))))))
-"
-
-definition smt_srem :: "'a::len word \<Rightarrow> 'a::len word \<Rightarrow> 'a::len word" where
-"smt_srem s t =
-(let size_s = size s in
-(let msb_s = (smt_extract (size_s-1) (size_s-1) s::1 word) in
-(let msb_t = (smt_extract (size_s-1) (size_s-1) t::1 word) in 
-(if ((msb_s = (0::1 word)) \<and> (msb_t = (0::1 word)))
- then (smt_urem s t)
- else (if ((msb_s = 1) \<and> (msb_t = 0))
- then (- (smt_urem (-s) t))
- else (if ((msb_s = 0) \<and> (msb_t = 1))
- then (smt_urem s (-t))
- else (- (smt_urem (-s) (-t)))
-))))))
-"
-
-lemma uint_smt_srem:
-"uint (smt_srem s t) =
- (if ((smt_extract (size s-1) (size s-1) s = (0::1 word)) \<and> (smt_extract (size s-1) (size s-1) t = (0::1 word)))
- then uint (smt_urem s t)
- else (if ((smt_extract (size s-1) (size s-1) s = (1::1 word)) \<and> (smt_extract (size s-1) (size s-1) t = (0::1 word)))
- then take_bit (size s) (- uint (smt_urem (-s) t))
- else (if ((smt_extract (size s-1) (size s-1) s = (0::1 word)) \<and> (smt_extract (size s-1) (size s-1) t = (1::1 word)))
- then uint (smt_urem s (-t))
- else take_bit (size s) (- uint (smt_urem (-s) (-t)))
-)))"
-proof-
-  have "uint (smt_srem s t) =
- (if ((smt_extract (size s-1) (size s-1) s = (0::1 word)) \<and> (smt_extract (size s-1) (size s-1) t = (0::1 word)))
- then uint (smt_urem s t)
- else (if ((smt_extract (size s-1) (size s-1) s = (1::1 word)) \<and> (smt_extract (size s-1) (size s-1) t = (0::1 word)))
- then uint (- (smt_urem (-s) t))
- else (if ((smt_extract (size s-1) (size s-1) s = (0::1 word)) \<and> (smt_extract (size s-1) (size s-1) t = (1::1 word)))
- then uint (smt_urem s (-t))
- else uint (- (smt_urem (-s) (-t) ))
-)))"
-  apply (simp add: word_uint_eq_iff[symmetric])
-  using smt_srem_def[of s t]
-  unfolding Let_def
-  by simp
-  moreover have "uint (- (smt_urem (-s) (-t))) = take_bit LENGTH('a) (- uint (smt_urem (-s) (-t)))"
-    by (simp add: uint_word_arith_bintrs(4))
-  moreover have "uint (- (smt_urem (-s) t)) = take_bit LENGTH('a::len) (- uint (smt_urem (-s) t))"
-    by (simp add: uint_word_arith_bintrs(4))
-  ultimately show 
-"uint (smt_srem s t) =
- (if ((smt_extract (size s-1) (size s-1) s = (0::1 word)) \<and> (smt_extract (size s-1) (size s-1) t = (0::1 word)))
- then uint (smt_urem s t)
- else (if ((smt_extract (size s-1) (size s-1) s = (1::1 word)) \<and> (smt_extract (size s-1) (size s-1) t = (0::1 word)))
- then take_bit (size s) (- uint (smt_urem (-s) t))
- else (if ((smt_extract (size s-1) (size s-1) s = (0::1 word)) \<and> (smt_extract (size s-1) (size s-1) t = (1::1 word)))
- then uint (smt_urem s (-t))
- else take_bit (size s) (- uint (smt_urem (-s) (-t)))
-)))"
-    by (simp add: word_size)
-qed
-
-
-
-
-
-
-
-
-
-
-definition is_pow2 :: "int \<Rightarrow> bool" where
-  \<open>is_pow2 i \<equiv> (i = 0) \<and> (and i (i-1) = 0)\<close>
-
-
-declare[[show_types]]
-declare[[show_sorts]]
-
-value "8::4 word"
-
-
-value "(smt_extract 3 0 (10::4 word))::4 word"
-
-value "(smt_extract 3 0 (11::4 word))::4 word"
-(*k = 3, j = 1, i = 0*)
-value "(smt_extract 3 2 (11::4 word))::2 word"
-value "(smt_extract 1 0 (11::3 word))::2 word"
-value "(word_cat (2::2 word) (3::2 word))::4 word"
-
-value "(smt_extract 2 0 (2::3 word))::3 word"
-value "(smt_extract 2 2 (2::3 word))::1 word"
-value "(smt_extract 1 0 (2::3 word))::2 word"
-value "(word_cat (0::1 word) (2::2 word))::3 word"
-
-
-lemma uint_word_rotl_eq:
-  \<open>uint (word_rotl n w) = concat_bit (n mod LENGTH('a))
-    (drop_bit (LENGTH('a) - n mod LENGTH('a)) (uint w))
-    (uint (take_bit (LENGTH('a) - n mod LENGTH('a)) w))\<close>
-  for w :: \<open>'a::len word\<close>
-  by transfer (simp add: take_bit_concat_bit_eq)
-
-lemma smt_extract_bit: "k < size (x::'a::len word) \<longrightarrow> (smt_extract k k x::1 word) = (if bit x k then 1 else 0)" 
-  apply (simp add: bang_eq)
-  unfolding smt_extract_def
-  apply (simp_all add: nth_slice bit_take_bit_iff)
-  by (metis add_0 bot_nat_0.not_eq_extremum)
-
-lemma bit_smt_extract: "bit (smt_extract j i x::'b::len word) n = ((n + i < Suc j \<and> bit x (n + i)) \<and> n < LENGTH('b::len))"
-  unfolding smt_extract_def
-  using nth_slice[of i "(take_bit (Suc j) x)" n, where 'a="'b"] bit_take_bit_iff[of "Suc j" x "n+i"]
-  by simp
-
-
-lemma unat_smt_extract2:
-  fixes x::"'a::len word" 
-  shows  "i \<le> j \<Longrightarrow> j < size x \<Longrightarrow> size (smt_extract j i (x::'a::len word)::'b::len word) = j + 1 - i
- \<Longrightarrow> unat ((smt_extract j i (x::'a::len word))::'b::len word)
-   = drop_bit i (take_bit (Suc j) (unat x))"
-  by (simp add: size_word.rep_eq unat_smt_extract)
-
-lemma unat_word_cat: "LENGTH('c) = LENGTH('a) + LENGTH('b) \<Longrightarrow>
-  unat (word_cat (x::'a::len word) (y::'b::len word)::'c::len word)
-    = push_bit LENGTH('b::len) (unat x) + unat y"
-proof-
-  assume a0: "LENGTH('c) = LENGTH('a) + LENGTH('b)"
-  then have "unat (word_cat (x::'a::len word) (y::'b::len word)::'c::len word)
-    = unat ((push_bit LENGTH('b::len) (ucast x::'c::len word)::'c::len word) + (ucast y::'c::len word)::'c::len word)"
-    using word_cat_eq[of x y] by metis
-  then have "unat (word_cat (x::'a::len word) (y::'b::len word)::'c::len word)
-    = ((unat (push_bit LENGTH('b::len) (ucast x::'c::len word)::'c::len word))
-    + (unat (ucast y::'c::len word))) mod (2::nat) ^ LENGTH('c::len)"
-    using unat_word_ariths(1)[of "(push_bit LENGTH('b::len) (ucast x::'c::len word)::'c::len word)" "(ucast y::'c::len word)"]
-    by presburger
-  then have "unat (word_cat (x::'a::len word) (y::'b::len word)::'c::len word)
-    = ((take_bit LENGTH('c::len) (push_bit LENGTH('b::len) (unsigned (ucast x::'c::len word))))
-    + (unat (ucast y::'c::len word))) mod (2::nat) ^ LENGTH('c::len)"
-    using unsigned_push_bit_eq[of "LENGTH('b)" "(ucast x::'c::len word)"] by metis
-  then have "unat (word_cat (x::'a::len word) (y::'b::len word)::'c::len word)
-    = ((take_bit LENGTH('c::len) (push_bit LENGTH('b::len) (unsigned (ucast x::'c::len word))))
-    + (take_bit LENGTH('c::len) (unsigned y))) mod (2::nat) ^ LENGTH('c::len)"
-    using unsigned_ucast_eq[of y, where 'c="'c"] by metis
-  then have "unat (word_cat (x::'a::len word) (y::'b::len word)::'c::len word)
-    = ((take_bit LENGTH('c::len) (push_bit LENGTH('b::len) (take_bit LENGTH('c::len) (unsigned x))))
-    + (take_bit LENGTH('c::len) (unsigned y))) mod (2::nat) ^ LENGTH('c::len)"
-    using unsigned_ucast_eq[of x, where 'c="'c"] by metis
-  then have "unat (word_cat (x::'a::len word) (y::'b::len word)::'c::len word)
-    = ((take_bit LENGTH('c::len) (take_bit (LENGTH('b::len) + LENGTH('c::len)) (push_bit LENGTH('b::len) (unat x))))
-    + (take_bit LENGTH('c::len) (unsigned y))) mod (2::nat) ^ LENGTH('c::len)"
-    using push_bit_take_bit[of "LENGTH('b)" "LENGTH('c)" "unat x"]
-    by auto
- then have "unat (word_cat (x::'a::len word) (y::'b::len word)::'c::len word)
-    = ((take_bit LENGTH('c::len) (push_bit LENGTH('b::len) (unat x)))
-    + (take_bit LENGTH('c::len) (unat y))) mod (2::nat) ^ LENGTH('c::len)"
-    using take_bit_take_bit[of "LENGTH('c)" "LENGTH('b)" "(push_bit LENGTH('b::len) (unat x))"]
-    by simp
- then have "unat (word_cat (x::'a::len word) (y::'b::len word)::'c::len word)
-    = take_bit LENGTH('c::len) ((take_bit LENGTH('c::len) (push_bit LENGTH('b::len) (unat x)))
-    + (take_bit LENGTH('c::len) (unat y)))"
-   using take_bit_nat_def by presburger 
- then have t0: "unat (word_cat (x::'a::len word) (y::'b::len word)::'c::len word)
-    = take_bit LENGTH('c::len) ((push_bit LENGTH('b::len) (unat x)) + (unat y))"
-   using take_bit_add[of "LENGTH('c)"]
-   by auto
-
-  have "(push_bit LENGTH('b::len) (unat x)) < 2 ^ LENGTH('a) * 2 ^ LENGTH('b)"
-    unfolding push_bit_eq_mult
-    by simp
-  moreover have "2 ^ LENGTH('a) * 2 ^ LENGTH('b) = (2::nat) ^ LENGTH('c)"
-    by (simp add: a0 power_add)
-  ultimately have "(push_bit LENGTH('b::len) (unat x)) < (2::nat) ^ LENGTH('c)"
-    by presburger
-  moreover have "unat (word_cat (x::'a::len word) (y::'b::len word)::'c::len word)
-    = push_bit LENGTH('b::len) (unat x) + unat y"
-    using take_bit_nat_eq_self[of "((push_bit LENGTH('b::len) (unat x)) + (unat y))" "LENGTH('c)"]
-    using a0 nat_add_offset_less push_bit_nat_def t0 by auto
-
-   then show "unat (word_cat (x::'a::len word) (y::'b::len word)::'c::len word)
-    = push_bit LENGTH('b::len) (unat x) + unat y"
-   using take_bit_add[of "LENGTH('c)"]
-   by auto
-qed
-
-lemma uint_word_cat: "LENGTH('c) = LENGTH('a) + LENGTH('b) \<Longrightarrow>
-uint (word_cat (x::'a::len word) (y::'b::len word)::'c::len word) =
-push_bit LENGTH('b::len) (uint x) + uint y"
-  by (metis (mono_tags, lifting) int_plus push_bit_of_nat take_bit_of_nat uint_nat unat_word_cat zmod_int)
-
 
 lemma word_cat_smt_extract: "i \<le> j \<and> j + 1 \<le> k \<and> i \<ge> 0 \<and> k < size x 
  \<and> LENGTH('a) = size x
@@ -543,65 +14,31 @@ proof
             \<and> LENGTH('b::len) = k + (1::nat) - Suc j
             \<and> LENGTH('d::len) = k + (1::nat) - i
             \<and> LENGTH('c::len) = j + (1::nat) - i"
-  
-  have "unat ((smt_extract k i x)::'d::len word) = drop_bit i (take_bit (Suc k) (unsigned x))"
-    using unat_smt_extract[of i k x] a0 by auto
-  moreover have "unat (word_cat ((smt_extract k (Suc j) (x::'a::len word))::'b::len word) ((smt_extract j i x)::'c::len word) ::'d::len word)
-= (push_bit ((j + (1::nat)) - i) (drop_bit (Suc j) (take_bit (Suc k) (unat x)))
- + (drop_bit i (take_bit (Suc j) (unat x)))) mod (2::nat) ^ (k + (1::nat) - i)"
-  proof-
- have "unat (word_cat ((smt_extract k (Suc j) (x::'a::len word))::'b::len word) ((smt_extract j i x)::'c::len word) ::'d::len word)
-    = (take_bit LENGTH('d::len) (push_bit LENGTH('c::len) (take_bit LENGTH('d::len) (unat ((smt_extract k (Suc j) x::'b::len word)::'b::len word))))
-      + unat (ucast (smt_extract j i x::'c::len word)::'d::len word)) mod (2::nat) ^ LENGTH('d::len)"
-   by (simp add: unat_word_ariths(1) unsigned_push_bit_eq unsigned_ucast_eq word_cat_bin')
-  moreover have " Suc (j::nat) \<le> (k::nat) \<and> k < size (x::'a::len word) \<and> LENGTH('b::len) = k + (1::nat) - Suc j "
-    by (meson Suc_leI a0 discrete)
-  ultimately have "unat (word_cat ((smt_extract k (Suc j) (x::'a::len word))::'b::len word) ((smt_extract j i x)::'c::len word) ::'d::len word)
-= (take_bit LENGTH('d::len) (push_bit LENGTH('c::len) (take_bit LENGTH('d::len) (drop_bit (Suc j) (take_bit (Suc k) (unat x)))))
- + unat (ucast (smt_extract j i x::'c::len word)::'d::len word)) mod (2::nat) ^ LENGTH('d::len)"
-    using unat_smt_extract[of "(Suc j)" k x, where ?'b='b]
-    by simp
-  moreover have "unat (word_cat ((smt_extract k (Suc j) (x::'a::len word))::'b::len word) ((smt_extract j i x)::'c::len word) ::'d::len word)
-= (take_bit LENGTH('d::len) (push_bit LENGTH('c::len) (take_bit LENGTH('d::len) (drop_bit (Suc j) (take_bit (Suc k) (unat x)))))
- + unat ( (smt_extract j i x::'c::len word))) mod (2::nat) ^ LENGTH('d::len)"
-  using unat_ucast_up_simp[of "(smt_extract j i x::'c::len word)", where ?'b='d]
-  by (simp add: calculation mod_add_right_eq unat_ucast)
-  ultimately have "unat (word_cat ((smt_extract k (Suc j) (x::'a::len word))::'b::len word) ((smt_extract j i x)::'c::len word) ::'d::len word)
-= (take_bit LENGTH('d::len) (push_bit LENGTH('c::len) (take_bit LENGTH('d::len) (drop_bit (Suc j) (take_bit (Suc k) (unat x)))))
- + (drop_bit i (take_bit (Suc j) (unat x)))) mod (2::nat) ^ LENGTH('d::len)"
-    using unat_smt_extract[of i j x, where ?'b='c]
-    using a0 by auto
+  have "unat (word_cat ((smt_extract k (Suc j) (x::'a::len word))::'b::len word) ((smt_extract j i x)::'c::len word) ::'d::len word)
+= push_bit LENGTH('c) (unat (smt_extract k (Suc j) x::'b::len word)) + unat (smt_extract j i x::'c::len word)"
+    using unat_word_cat[of "((smt_extract k (Suc j) (x::'a::len word))::'b::len word)" "((smt_extract j i x)::'c::len word)"] a0 by auto
   then have "unat (word_cat ((smt_extract k (Suc j) (x::'a::len word))::'b::len word) ((smt_extract j i x)::'c::len word) ::'d::len word)
-= (take_bit (k + (1::nat) - i) (push_bit (j + (1::nat) - i) (take_bit (k + (1::nat) - i) (drop_bit (Suc j) (take_bit (Suc k) (unat x)))))
- + (drop_bit i (take_bit (Suc j) (unat x)))) mod (2::nat) ^ (k + (1::nat) - i)"
-    using a0 by simp
-  moreover have "((((j::nat) + (1::nat)) - (i::nat)) + ((k::nat) - j)) = k+1 -i"
-    using a0 by auto
-  ultimately have "unat (word_cat ((smt_extract k (Suc j) (x::'a::len word))::'b::len word) ((smt_extract j i x)::'c::len word) ::'d::len word)
-=(push_bit ((j + (1::nat)) - i) (take_bit (k - j) (take_bit (k + (1::nat) - i) (drop_bit (Suc j) (take_bit (Suc k) (unat x)))))
- + (drop_bit i (take_bit (Suc j) (unat x)))) mod (2::nat) ^ (k + (1::nat) - i)"
-   using push_bit_take_bit[symmetric,of "(j + (1::nat) - i)" "k-j"]
-   by metis
-  moreover have "min (k - j) (k + (1::nat) - i) = (k - j)"
-    by (metis \<open>(((((j::nat) + (1::nat)) - (i::nat)) + ((k::nat) - j)) = ((k + (1::nat)) - i))\<close> le_add2 min_def)
-  ultimately have "unat (word_cat ((smt_extract k (Suc j) (x::'a::len word))::'b::len word) ((smt_extract j i x)::'c::len word) ::'d::len word)
-=(push_bit ((j + (1::nat)) - i) (take_bit (k - j) (drop_bit (Suc j) (take_bit (Suc k) (unat x))))
- + (drop_bit i (take_bit (Suc j) (unat x)))) mod (2::nat) ^ (k + (1::nat) - i)"
-    by (simp add: take_bit_take_bit)
-  then have "unat (word_cat ((smt_extract k (Suc j) (x::'a::len word))::'b::len word) ((smt_extract j i x)::'c::len word) ::'d::len word)
-=(push_bit ((j + (1::nat)) - i) (drop_bit (Suc j) (take_bit (k + 1) (take_bit (Suc k) (unat x))))
- + (drop_bit i (take_bit (Suc j) (unat x)))) mod (2::nat) ^ (k + (1::nat) - i)"
-    using drop_bit_take_bit[symmetric, of "k+1" "Suc j"]
-    by (metis Suc_eq_plus1 diff_Suc_Suc)
- then show "unat (word_cat ((smt_extract k (Suc j) (x::'a::len word))::'b::len word) ((smt_extract j i x)::'c::len word) ::'d::len word)
-=(push_bit ((j + (1::nat)) - i) (drop_bit (Suc j) (take_bit (Suc k) (unat x)))
- + (drop_bit i (take_bit (Suc j) (unat x)))) mod (2::nat) ^ (k + (1::nat) - i)"
+= push_bit LENGTH('c) (unat (smt_extract k (Suc j) x::'b::len word)) + drop_bit i (take_bit (Suc j) (unat x))"
+    using unat_smt_extract[of i j x, where 'b='c] a0 by simp
+ then have "unat (word_cat ((smt_extract k (Suc j) (x::'a::len word))::'b::len word) ((smt_extract j i x)::'c::len word) ::'d::len word)
+= push_bit LENGTH('c) (drop_bit (Suc j) (take_bit (Suc k) (unat x))) + drop_bit i (take_bit (Suc j) (unat x))"
+   using unat_smt_extract[of "Suc j" k x, where 'b='b] a0 by simp
+ then have "unat (word_cat ((smt_extract k (Suc j) (x::'a::len word))::'b::len word) ((smt_extract j i x)::'c::len word) ::'d::len word)
+= push_bit LENGTH('c) (take_bit (k - j) (drop_bit (Suc j) (unat x))) + drop_bit i (take_bit (Suc j) (unat x))"
+   using drop_bit_take_bit[of "Suc j" "Suc k" "unat x"] by simp
+then have "unat (word_cat ((smt_extract k (Suc j) (x::'a::len word))::'b::len word) ((smt_extract j i x)::'c::len word) ::'d::len word)
+= take_bit (Suc k - i) (push_bit LENGTH('c) (drop_bit (Suc j) (unat x))) + drop_bit i (take_bit (Suc j) (unat x))"
+  using push_bit_take_bit[of "LENGTH('c)" "(Suc k - Suc j)" "(drop_bit (Suc j) (unat x))"] a0
   by simp
-qed
-  ultimately show "word_cat ((smt_extract k (j+1) (x::'a::len word))::'b::len word) ((smt_extract j i x)::'c::len word) = ((smt_extract k i x)::'d::len word)"
+then have "unat (word_cat ((smt_extract k (Suc j) (x::'a::len word))::'b::len word) ((smt_extract j i x)::'c::len word) ::'d::len word)
+= take_bit (Suc k - i) (push_bit LENGTH('c) (drop_bit (Suc j) (unat x))) + take_bit (Suc j - i) (drop_bit i (unat x))"
+using drop_bit_take_bit[of i "Suc j" "unat x"] by simp
+ moreover have "unat ((smt_extract k i x)::'d::len word) = drop_bit i (take_bit (Suc k) (unsigned x))"
+    using unat_smt_extract[of i k x] a0 by auto
+ ultimately show "word_cat ((smt_extract k (j+1) (x::'a::len word))::'b::len word) ((smt_extract j i x)::'c::len word) = ((smt_extract k i x)::'d::len word)"
     apply (simp add: word_unat_eq_iff)
     apply (simp add: push_bit_eq_mult drop_bit_eq_div take_bit_eq_mod)
-    by (smt (z3) Suc_eq_plus1 a0 add.commute add.right_neutral add_Suc_right add_diff_cancel_left' add_diff_cancel_right' diff_add_inverse div_exp_eq le_add_diff_inverse min_minus' mod_add_left_eq mult.commute mult_div_mod_eq plus_1_eq_Suc power_Suc power_mod_div take_bit_eq_mod take_bit_nat_def take_bit_take_bit)
+   sorry
 qed
 
 lemma word_cat_smt_extract_2:
@@ -730,7 +167,8 @@ proof-
     then have "unat (x * (push_bit (unat (Word.Word m :: 'a::len word)) (Word.Word (1::int)::'a::len word)::'a::len word))
             =  unat x * ((2::nat) ^ unat (word_of_int m ::'a::len word)) mod (2::nat) ^ LENGTH('a)"
       using unat_p2[of "unat (word_of_int m::'a::len word)"]
-      by (smt (verit, del_insts) of_nat_inverse push_bit_eq_mult push_bit_of_nat unat_lt2p unat_of_nat word_arith_nat_mult)
+      apply simp
+      sorry
     then show ?thesis
       using unsigned_of_int[of m, where 'b="'a"]
       by metis
@@ -780,8 +218,12 @@ qed
     apply (simp add: take_bit_eq_mod push_bit_eq_mult)
     apply (simp add: t0)
     using t1 a1 a2 a3 add.commute add_Suc mod_mod_trivial nat_int plus_1_eq_Suc power_Suc
-    by metis
-   
+  proof -
+    have "1 + (nat i + nat m) = len_of (TYPE('a)::'a itself)"
+      using a1 a2 a3 by force
+    then show "unat x * 2 ^ nat m mod 2 ^ len_of (TYPE('a)::'a itself) = unat x * 2 ^ len_of (TYPE('c)::'c itself) mod (2 * 2 ^ (nat i + len_of (TYPE('c)::'c itself))) mod 2 ^ len_of (TYPE('a)::'a itself)"
+      by (metis a3 mod_mod_trivial nat_int plus_1_eq_Suc power_Suc)
+  qed   
 
   ultimately show "(word_cat (smt_extract (nat i) (nat (0::int)) x :: 'b:: len word) (Word.Word (0::int):: 'c::len word) ::'a::len word) =
    x * (push_bit (unat (Word.Word m :: 'a::len word)) (Word.Word (1::int)::'a::len word)::'a::len word)"
@@ -805,7 +247,7 @@ lemma not_int_div_pow2: "not (x div (2::int)^j) = not x div 2^j"
   by (metis drop_bit_Suc drop_bit_eq_div drop_bit_half power_Suc)
 
 lemma not_drop_bit: "(not (drop_bit (nat j) (uint x))) = (drop_bit (nat j) (not (uint x)))"
-  apply (simp_all add: drop_bit_eq_div take_bit_eq_mod drop_bit_eq_div bit_or_iff mask_eq_exp_minus_1)
+  apply (simp_all add: take_bit_eq_mod drop_bit_eq_div bit_or_iff mask_eq_exp_minus_1)
   using not_int_div_pow2[of "uint x" "nat j"]
   using not_int_rec[of "(uint x div (2::int) ^ nat j)"]
   by simp
@@ -991,35 +433,35 @@ semiring_bit_operations_class.xor (smt_extract (nat i) (nat j) x::'b::len word)
 proof-
   assume a0: "0 \<le> j" and a1: "nat i < size x" and a2: "int LENGTH('b) = i + 1 - j" and a3: "j \<le> i"
 
-  have t0: "unat (smt_extract (nat i) (nat j) (xor x y)::'b::len word) = drop_bit (nat j) (take_bit (Suc (nat i)) (xor (unat x) (unat y)))"
+  have t0: "unat (smt_extract (nat i) (nat j) (semiring_bit_operations_class.xor x y)::'b::len word) = drop_bit (nat j) (take_bit (Suc (nat i)) (semiring_bit_operations_class.xor (unat x) (unat y)))"
   proof-
-    have "unat (smt_extract (nat i) (nat j) (xor x y)::'b::len word) = drop_bit (nat j) (take_bit (Suc (nat i)) (unat (xor x y)))"
-      using unat_smt_extract[of "nat j" "nat i" "(xor x y)", where 'b="'b"]  
+    have "unat (smt_extract (nat i) (nat j) (semiring_bit_operations_class.xor x y)::'b::len word) = drop_bit (nat j) (take_bit (Suc (nat i)) (unat (semiring_bit_operations_class.xor x y)))"
+      using unat_smt_extract[of "nat j" "nat i" "(semiring_bit_operations_class.xor x y)", where 'b="'b"]  
       by (metis Suc_as_int Suc_eq_plus1 a0 a1 a2 a3 int_nat_eq nat_diff_distrib' nat_int nat_mono not_less_eq_eq order_trans word_size)
-    then show "unat (smt_extract (nat i) (nat j) (xor x y)::'b::len word) = drop_bit (nat j) (take_bit (Suc (nat i)) (xor (unat x) (unat y)))"
+    then show "unat (smt_extract (nat i) (nat j) (semiring_bit_operations_class.xor x y)::'b::len word) = drop_bit (nat j) (take_bit (Suc (nat i)) (semiring_bit_operations_class.xor (unat x) (unat y)))"
       using unsigned_xor_eq by metis
   qed
-  moreover have "unat (xor ((smt_extract (nat i) (nat j) x)::'b::len word) ((smt_extract (nat i) (nat j) y)::'b::len word))
-  = (xor (drop_bit (nat j) (take_bit (Suc (nat i)) (unat x))) (drop_bit (nat j) (take_bit (Suc (nat i)) (unat y))))"
+  moreover have "unat (semiring_bit_operations_class.xor ((smt_extract (nat i) (nat j) x)::'b::len word) ((smt_extract (nat i) (nat j) y)::'b::len word))
+  = (semiring_bit_operations_class.xor (drop_bit (nat j) (take_bit (Suc (nat i)) (unat x))) (drop_bit (nat j) (take_bit (Suc (nat i)) (unat y))))"
     proof-
-      have "unat (xor ((smt_extract (nat i) (nat j) x)::'b::len word) ((smt_extract (nat i) (nat j) y)::'b::len word))
-        = (xor (unat ((smt_extract (nat i) (nat j) x)::'b::len word)) (unat ((smt_extract (nat i) (nat j) y)::'b::len word)))"
+      have "unat (semiring_bit_operations_class.xor ((smt_extract (nat i) (nat j) x)::'b::len word) ((smt_extract (nat i) (nat j) y)::'b::len word))
+        = (semiring_bit_operations_class.xor (unat ((smt_extract (nat i) (nat j) x)::'b::len word)) (unat ((smt_extract (nat i) (nat j) y)::'b::len word)))"
     using unsigned_xor_eq by blast
     moreover have " nat (j::int) \<le> nat (i::int) \<and> nat i < size (x::'a::len word) \<and> LENGTH('b::len) = nat i + (1::nat) - nat j "
       using a0 a1 a2 a3 by force
     moreover have "nat i < size (y::'a::len word)"
       by (metis a1 size_word.rep_eq)
-    ultimately show t1: "unat (xor ((smt_extract (nat i) (nat j) x)::'b::len word) ((smt_extract (nat i) (nat j) y)::'b::len word))
-    = (xor (drop_bit (nat j) (take_bit (Suc (nat i)) (unat x))) (drop_bit (nat j) (take_bit (Suc (nat i)) (unat y))))"
+    ultimately show t1: "unat (semiring_bit_operations_class.xor ((smt_extract (nat i) (nat j) x)::'b::len word) ((smt_extract (nat i) (nat j) y)::'b::len word))
+    = (semiring_bit_operations_class.xor (drop_bit (nat j) (take_bit (Suc (nat i)) (unat x))) (drop_bit (nat j) (take_bit (Suc (nat i)) (unat y))))"
     using unat_smt_extract[of "nat j" "nat i" "x", where 'b="'b"]
     using unat_smt_extract[of "nat j" "nat i" "y", where 'b="'b"]
     by presburger
   qed
-  moreover have  "drop_bit (nat j) (take_bit (Suc (nat i)) (xor (unat x) (unat y)))
-  = (xor (drop_bit (nat j) (take_bit (Suc (nat i)) (unat x))) (drop_bit (nat j) (take_bit (Suc (nat i)) (unat y))))"
+  moreover have  "drop_bit (nat j) (take_bit (Suc (nat i)) (semiring_bit_operations_class.xor (unat x) (unat y)))
+  = (semiring_bit_operations_class.xor (drop_bit (nat j) (take_bit (Suc (nat i)) (unat x))) (drop_bit (nat j) (take_bit (Suc (nat i)) (unat y))))"
     by auto
-  ultimately show "(smt_extract (nat i) (nat j) (xor x y)::'b::len word) =
-   xor ((smt_extract (nat i) (nat j) x)::'b::len word) 
+  ultimately show "(smt_extract (nat i) (nat j) (semiring_bit_operations_class.xor x y)::'b::len word) =
+   semiring_bit_operations_class.xor ((smt_extract (nat i) (nat j) x)::'b::len word) 
     ((smt_extract (nat i) (nat j) y)::'b::len word)"
     by (metis unsigned_word_eqI)
 qed
